VisualProof/Diagram/Concrete/Subgraph.lean
@@ -1,2 +1,5 @@
 import VisualProof.Diagram.Concrete.Subgraph.Selection
 import VisualProof.Diagram.Concrete.Subgraph.Reindex
+import VisualProof.Diagram.Concrete.Subgraph.Remove
+import VisualProof.Diagram.Concrete.Subgraph.Extract
+import VisualProof.Diagram.Concrete.Subgraph.Decomposition
